Crypto.AE* : Created vs. Coerced

src/tls/Crypto.AEAD.fst
@@ -20,7 +20,7 @@ open Declassify
 noeq
 inline_for_extraction
 type cstate
-  (a: SC.supported_alg) (phi: plain_pred)
+  (a: SC.supported_alg)
 = {
   ec: B.pointer (EC.state_s a);
   kv: G.erased (SC.kv a);
@@ -30,78 +30,109 @@ type cstate
 let mphi (phi: plain_pred) : Tot (Model.plain_pred) =
   phi
 
-let state (a: SC.supported_alg) (phi: plain_pred) =
-  if F.model
-  then Model.state a (mphi phi)
-  else cstate a phi
-
+noeq
 inline_for_extraction
+type state (a: SC.supported_alg) (phi: plain_pred) =
+  // trick for extraction instead of using refinement
+  | Created: (log: (if F.model then Model.state a phi else squash False)) -> state a phi
+  | Coerced: (st: cstate a) -> state a phi
+
+let safe #a #phi s =
+  F.model && Created? s
+
 noextract
-let state_m
-  (#a: SC.supported_alg) (#phi: plain_pred) (s: state a phi { F.model == true })
-: Tot (Model.state a (mphi phi))
-= s
-
-inline_for_extraction
-let state_ec
-  (#a: SC.supported_alg) (#phi: plain_pred)
-  (s: state a phi { F.model == false })
-: Tot (B.pointer (EC.state_s a))
-= (s <: cstate a phi).ec
+let log (#a: _) (#phi: _) (s: state a phi { safe s }) : Tot (Model.state a phi)
+= Created?.log s
 
 let state_kv
   (#a: SC.supported_alg) (#phi: plain_pred)
   (s: state a phi)
 : GTot (SC.kv a)
-= if F.model then Model.state_kv (state_m s) else G.reveal (s <: cstate a phi).kv
+= if safe s
+  then Model.state_kv (log s)
+  else match s with
+  | Coerced st -> G.reveal st.kv
 
 unfold
 let invariant' (#a: SC.supported_alg) (#phi: plain_pred) (h: HS.mem) (s: state a phi) : GTot Type0 =
-  if F.model
-  then
-    Model.invariant h (state_m s)
-  else
-    EC.invariant h (state_ec s) /\
-    EC.footprint h (state_ec s) == Ghost.reveal (s <: cstate a phi).fp /\
-    EC.freeable h (state_ec s) /\
-    EC.as_kv (B.deref h (state_ec s)) == state_kv s
+  if safe s
+  then Model.invariant h (log s)
+  else match s with
+  | Coerced st ->
+    EC.invariant h st.ec /\
+    EC.footprint h st.ec == Ghost.reveal st.fp /\
+    EC.freeable h st.ec /\
+    EC.as_kv (B.deref h st.ec) == state_kv s
 
 let invariant = invariant'
 
 let footprint (#a: SC.supported_alg) (#phi: plain_pred) (s: state a phi) : GTot B.loc =
-  if F.model
-  then
-    Model.footprint (state_m s)
-  else
-    Ghost.reveal (s <: cstate a phi).fp
+  if safe s
+  then Model.footprint (log s)
+  else match s with
+  | Coerced st -> Ghost.reveal st.fp
 
 let frame_invariant
   #a #phi h s l h'
-= if F.model
-  then
-    Model.frame_invariant h (state_m s) l h'
-  else begin
-    EC.frame_invariant l (state_ec s) h h'
-  end
+= if safe s
+  then Model.frame_invariant h (log s) l h'
+  else match s with
+  | Coerced st -> EC.frame_invariant l st.ec h h'
+
+let sample a k =
+  Random.sample_secret_buffer (U32.uint_to_t (SC.key_length a)) k
+
+let coerce r a k phi = 
+    let h0 = HST.get () in
+    let dst : B.pointer (B.pointer_or_null (EC.state_s a)) = B.mmalloc r B.null 1ul in // I could also allocate it onto a fresh stack frame, but it's useless here
+    let h1 = HST.get () in
+    let res =
+      match EC.create_in r dst k with
+      | EE.UnsupportedAlgorithm ->
+        B.free dst;
+        None
+      | EE.Success ->
+        let h2 = HST.get () in
+        let b : B.pointer (EC.state_s a) = B.index dst 0ul in
+        let s : state a phi = Coerced ({ec = b; kv = G.hide (B.as_seq h0 k); fp = G.hide (EC.footprint h2 b)}) in        
+        B.free dst;
+        let h3 = HST.get () in
+        frame_invariant h2 s (B.loc_addr_of_buffer dst) h3;
+        Some s
+    in
+    let h4 = HST.get () in
+    B.modifies_only_not_unused_in B.loc_none h0 h4;
+    res
+
+let create r a k phi = 
+    sample a k;
+    let kv = MU.get_buffer k (U32.uint_to_t (SC.key_length a)) in
+    let res = Created (Model.create r kv (mphi phi) <: Model.state a (mphi phi)) in
+    res
 
 let fresh_iv
   #a #phi h s iv
-= F.model == true ==> Model.fresh_iv h (state_m s) iv
+= safe s ==> Model.fresh_iv h (log s) iv
 
 let frame_fresh_iv
   #a #phi h s iv l h'
-= if F.model
-  then Model.frame_fresh_iv h (state_m s) iv l h'
+= if safe s
+  then Model.frame_fresh_iv h (log s) iv l h'
+  else ()
 
 let is_fresh_iv
   #a #phi s iv
-= let h = HST.get () in
-  let iv_s = MU.get_buffer iv iv_len in
-  let h1 = HST.get () in
-  frame_invariant h s B.loc_none h1;
-  let res = Model.is_fresh_iv (state_m s) iv_s in
-  frame_fresh_iv h s iv_s B.loc_none h1 ;
-  res
+= if safe s
+  then
+    let log = log s in
+    let h = HST.get () in
+    let iv_s = MU.get_buffer iv iv_len in
+    let h1 = HST.get () in
+    frame_invariant h s B.loc_none h1;
+    let res = Model.is_fresh_iv log iv_s in
+    frame_fresh_iv h s iv_s B.loc_none h1;
+    res
+  else true
 
 // TODO: move to EverCrypt.AEAD
 noextract
@@ -122,9 +153,8 @@ let tag_len : (x: SC.alg) -> Tot (y: U32.t { U32.v y == SC.tag_length x }) =
 let encrypt #a #phi s plain plain_len cipher = 
   let h0 = HST.get () in
   let iv = B.sub cipher 0ul iv_len in
-  if F.model
-  then begin
-    let s : Model.state a (mphi phi) = s in
+  if safe s then
+    let s = log s in
     let iv_s = MU.get_buffer iv iv_len in
     let plain_s = MU.get_buffer plain plain_len in
     let cipher_tag_len = plain_len `U32.add` tag_len a in
@@ -137,7 +167,8 @@ let encrypt #a #phi s plain plain_len cipher =
     MU.put_buffer cipher_tag' cipher_tag_len cipher_s;
     let h3 = HST.get () in
     Model.frame_invariant h2 s (B.loc_buffer cipher_tag') h3
-  end else begin
+  else match s with
+  | Coerced st ->
     // E.random_sample iv_len iv; // TODO
     let ad = B.sub iv 0ul 0ul in
     let ad_len = 0ul in
@@ -145,7 +176,7 @@ let encrypt #a #phi s plain plain_len cipher =
     let tag' = B.sub cipher (iv_len `U32.add` plain_len) (tag_len a) in
     let _ = EC.encrypt
       #(G.hide a)
-      (state_ec s)
+      st.ec
       iv
       iv_len
       ad
@@ -157,22 +188,20 @@ let encrypt #a #phi s plain plain_len cipher =
     in
     let h' = HST.get () in
     assert (B.as_seq h' (B.gsub cipher iv_len (B.len cipher `U32.sub` iv_len)) `Seq.equal` Seq.append (B.as_seq h' cipher') (B.as_seq h' tag'))
-  end
 
 let decrypt #a #phi s cipher cipher_len plain = 
   let h0 = HST.get () in
   let iv = B.sub cipher 0ul iv_len in
   let plain_len = cipher_len `U32.sub` tag_len a `U32.sub` iv_len in
-  if F.model = true
-  then begin
-    let s : Model.state a (mphi phi) = s in
+  if safe s then
+    let s = log s in
     let iv_s = MU.get_buffer iv iv_len in
     let cipher_tag_len = cipher_len `U32.sub` iv_len in
     let cipher_tag = B.sub cipher iv_len cipher_tag_len in
     let cipher_tag_s = MU.get_buffer cipher_tag cipher_tag_len in
     let h1 = HST.get () in
     Model.frame_invariant h0 s B.loc_none h1;
-    match Model.decrypt s iv_s cipher_tag_s with
+    begin match Model.decrypt s iv_s cipher_tag_s with
     | None -> EE.AuthenticationFailure
     | Some plain_s ->
       let h2 = HST.get () in
@@ -180,7 +209,9 @@ let decrypt #a #phi s cipher cipher_len plain =
       let h3 = HST.get () in
       Model.frame_invariant h2 s (B.loc_buffer plain) h3;
       EE.Success
-  end else begin
+    end
+  else match s with
+  | Coerced st ->
     let ad = B.sub iv 0ul 0ul in
     let ad_len = 0ul in
     let cipher' = B.sub cipher iv_len plain_len in
@@ -188,7 +219,7 @@ let decrypt #a #phi s cipher cipher_len plain =
     let h = HST.get () in
     let res = EC.decrypt
       #(G.hide a)
-      (state_ec s)
+      st.ec
       iv
       iv_len
       ad
@@ -201,40 +232,12 @@ let decrypt #a #phi s cipher cipher_len plain =
     assert (B.as_seq h (B.gsub cipher iv_len (B.len cipher `U32.sub` iv_len)) `Seq.equal` Seq.append (B.as_seq h cipher') (B.as_seq h tag'));
     let h' = HST.get () in
     res
-  end
 
 #pop-options
 
-let create r #a k phi = 
-  if F.model
-  then
-    let kv = MU.get_buffer k (U32.uint_to_t (SC.key_length a)) in
-    let res = Model.create r kv (mphi phi) <: Model.state a (mphi phi) in
-    Some res
-  else begin
-    let h0 = HST.get () in
-    let dst : B.pointer (B.pointer_or_null (EC.state_s a)) = B.mmalloc r B.null 1ul in // I could also allocate it onto a fresh stack frame, but it's useless here
-    let h1 = HST.get () in
-    let res =
-      match EC.create_in r dst k with
-      | EE.UnsupportedAlgorithm ->
-        B.free dst;
-        None
-      | EE.Success ->
-        let h2 = HST.get () in
-        let b : B.pointer (EC.state_s a) = B.index dst 0ul in
-        let s : state a phi = {ec = b; kv = G.hide (B.as_seq h0 k); fp = G.hide (EC.footprint h2 b)} <: cstate a phi in        
-        B.free dst;
-        let h3 = HST.get () in
-        frame_invariant h2 s (B.loc_addr_of_buffer dst) h3;
-        Some s
-    in
-    let h4 = HST.get () in
-    B.modifies_only_not_unused_in B.loc_none h0 h4;
-    res
-  end
-
 let free #a #phi s = 
-  if F.model
-  then Model.free (state_m s)
-  else EC.free #(G.hide a) (state_ec s)
+  if safe s
+  then Model.free (log s)
+  else match s with
+  | Coerced st ->
+    EC.free #(G.hide a) st.ec
